@prefix rdf: <http://www.w3.org/1999/02/22-rdf-syntax-ns#> .
@prefix rdfs: <http://www.w3.org/2000/01/rdf-schema#> .
@prefix dc: <http://purl.org/dc/elements/1.1/> .
@prefix owl: <http://www.w3.org/2002/07/owl#> .
@prefix xml: <http://www.w3.org/XML/1998/namespace> .
@prefix xsd: <http://www.w3.org/2001/XMLSchema#> .
@prefix mel: <https://jgeldart.github.io/pinafore/mel#> .

mel: a owl:Ontology;
  dc:title "Modal Expression Language 1.0";
  rdfs:comment """
  The Modal Expression Language is an extension to OWL 2 that provides vocabulary
  for describing situations and contexts. It tackles the following forms of
  modality:

  * State of knowledge (MKNF) including provability of knowledge.
  * Contingency in terms of necessity and possibility.
  * Cooperation and agency using STIT (Sees To It That) modals.
  * Temporal modality through LTL/PLTL.

  To support these, it also defines vocabulary for expressing richer property
  descriptions, nominal schemas, and vagueness through FuzzyDL.
  """;
  owl:imports owl:
  .


mel:cumulativeSubjectOver a rdf:Property;
  rdfs:label "cumulativeSubjectOver";
  rdfs:comment "The property that determines which property is cumulative over a plural collection in subject position.";
  rdfs:isDefinedBy mel:;
  rdfs:domain rdf:Property;
  rdfs:range rdf:Property
  .

mel:distributiveSubjectOver a rdf:Property;
  rdfs:label "distributiveSubjectOver";
  rdfs:comment "The property that determines which property is distributive over a plural collection in subject position.";
  rdfs:isDefinedBy mel:;
  rdfs:domain rdf:Property;
  rdfs:range rdf:Property
  .

mel:cumulativeObjectOver a rdf:Property;
  rdfs:label "cumulativeObjectOver";
  rdfs:comment "The property that determines which property is cumulative over a plural collection in object position.";
  rdfs:isDefinedBy mel:;
  rdfs:domain rdf:Property;
  rdfs:range rdf:Property
  .

mel:distributiveObjectOver a rdf:Property;
  rdfs:label "distributiveObjectOver";
  rdfs:comment "The property that determines which property is distributive over a plural collection in object position.";
  rdfs:isDefinedBy mel:;
  rdfs:domain rdf:Property;
  rdfs:range rdf:Property
  .

mel:propertyIntersectionOf a rdf:Property;
  rdfs:label "propertyIntersectionOf";
  rdfs:comment "The property that determines the collection of object or datatype properties that build an intersection.";
  rdfs:isDefinedBy mel:;
  rdfs:domain rdf:Property;
  rdfs:range rdf:List
  .

mel:propertyUnionOf a rdf:Property;
  rdfs:label "propertyUnionOf";
  rdfs:comment "The property that determines the collection of object or datatype properties that build a union.";
  rdfs:isDefinedBy mel:;
  rdfs:domain rdf:Property;
  rdfs:range rdf:List
  .

mel:propertyComplementOf a rdf:Property;
  rdfs:label "propertyComplementOf";
  rdfs:comment "The property that determines that a property is the complement of another property.";
  rdfs:isDefinedBy mel:;
  rdfs:domain rdf:Property;
  rdfs:range rdf:Property
  .

mel:propertyChainOf a rdf:Property;
  rdfs:label "propertyChainOf";
  rdfs:comment "The property that determines the sequence of object or datatype properties that build a chain of steps from first step to last.";
  rdfs:isDefinedBy mel:;
  rdfs:domain rdf:Property;
  rdfs:range rdf:List
  .

mel:hasIsA a owl:AnnotationProperty;
  rdfs:label "hasIsA";
  rdfs:comment "The property that determines the 'is a' property for a class.";
  rdfs:isDefinedBy mel:;
  rdfs:domain rdfs:Class;
  rdfs:range rdf:Property
  .
