@prefix rdf: <http://www.w3.org/1999/02/22-rdf-syntax-ns#> .
@prefix rdfs: <http://www.w3.org/2000/01/rdf-schema#> .
@prefix dc: <http://purl.org/dc/elements/1.1/> .
@prefix owl: <http://www.w3.org/2002/07/owl#> .
@prefix xml: <http://www.w3.org/XML/1998/namespace> .
@prefix xsd: <http://www.w3.org/2001/XMLSchema#> .
@prefix mel: <https://jgeldart.github.io/pinafore/mel#> .

mel: a owl:Ontology;
  dc:title "Modal Expression Language 1.0";
  rdfs:comment """
  The Modal Expression Language is an extension to OWL 2 that provides vocabulary
  for describing situations and contexts. It tackles the following forms of
  modality:

  * State of knowledge (MKNF) including provability of knowledge.
  * Contingency in terms of necessity and possibility.
  * Cooperation and agency using STIT (Sees To It That) modals.
  * Temporal modality through LTL/PLTL.

  To support these, it also defines vocabulary for expressing richer property
  descriptions, nominal schemas, and vagueness through FuzzyDL.
  """;
  owl:imports owl:
  .

mel:ModalRestriction a rdfs:Class;
  rdfs:label "ModalRestriction";
  rdfs:comment "The class of restrictions that operate over possible worlds.";
  rdfs:isDefinedBy mel:;
  rdfs:subClassOf owl:Restriction
  .

mel:StructuralModal a rdfs:Class;
  rdfs:label "StructuralModal";
  rdfs:comment "The class of modal restrictions where the accessibility relation is the argument structure.";
  rdfs:isDefinedBy mel:;
  rdfs:subClassOf mel:ModalRestriction
  .

mel:AlethicModal a rdfs:Class;
  rdfs:label "AlethicModal";
  rdfs:comment "The class of structural modals that quantify over possible worlds.";
  rdfs:isDefinedBy mel:;
  rdfs:subClassOf mel:StructuralModal
  .

mel:EpistemicModal a rdfs:Class;
  rdfs:label "EpistemicModal";
  rdfs:comment "The class of structural modals that quantify over knowledge of possible world.";
  rdfs:isDefinedBy mel:;
  rdfs:subClassOf mel:StructuralModal
  .

mel:DeonticModal a rdfs:Class;
  rdfs:label "DeonticModal";
  rdfs:comment "The class of structural modals that quantify over the agency responsible for asserting possible worlds.";
  rdfs:isDefinedBy mel:;
  rdfs:subClassOf mel:StructuralModal
  .

mel:TemporalModal a rdfs:Class;
  rdfs:label "TemporalModal";
  rdfs:comment "The class of modal restrictions where the accessibility relation is the induced temporal order.";
  rdfs:isDefinedBy mel:;
  rdfs:subClassOf mel:ModalRestriction
  .

mel:MembershipProperty a rdfs:Class;
  rdfs:label "MembershipProperty";
  rdfs:comment "The class of properties that may be plurally quantified over.";
  rdfs:isDefinedBy mel:;
  rdfs:subClassOf owl:ObjectProperty
  .

mel:IsAProperty a rdfs:Class;
  rdfs:label "IsAProperty";
  rdfs:comment "The class of properties that relate an individual to itself.";
  rdfs:isDefinedBy mel:;
  rdfs:subClassOf owl:ObjectProperty
  .

mel:cumulativeSubjectOver a rdf:Property;
  rdfs:label "cumulativeSubjectOver";
  rdfs:comment "The property that determines which property is cumulative over a plural collection in subject position.";
  rdfs:isDefinedBy mel:;
  rdfs:domain rdf:Property;
  rdfs:range rdf:Property
  .

mel:distributiveSubjectOver a rdf:Property;
  rdfs:label "distributiveSubjectOver";
  rdfs:comment "The property that determines which property is distributive over a plural collection in subject position.";
  rdfs:isDefinedBy mel:;
  rdfs:domain rdf:Property;
  rdfs:range rdf:Property
  .

mel:cumulativeObjectOver a rdf:Property;
  rdfs:label "cumulativeObjectOver";
  rdfs:comment "The property that determines which property is cumulative over a plural collection in object position.";
  rdfs:isDefinedBy mel:;
  rdfs:domain rdf:Property;
  rdfs:range rdf:Property
  .

mel:distributiveObjectOver a rdf:Property;
  rdfs:label "distributiveObjectOver";
  rdfs:comment "The property that determines which property is distributive over a plural collection in object position.";
  rdfs:isDefinedBy mel:;
  rdfs:domain rdf:Property;
  rdfs:range rdf:Property
  .

mel:propertyIntersectionOf a rdf:Property;
  rdfs:label "propertyIntersectionOf";
  rdfs:comment "The property that determines the collection of object or datatype properties that build an intersection.";
  rdfs:isDefinedBy mel:;
  rdfs:domain rdf:Property;
  rdfs:range rdf:List
  .

mel:propertyUnionOf a rdf:Property;
  rdfs:label "propertyUnionOf";
  rdfs:comment "The property that determines the collection of object or datatype properties that build a union.";
  rdfs:isDefinedBy mel:;
  rdfs:domain rdf:Property;
  rdfs:range rdf:List
  .

mel:propertyComplementOf a rdf:Property;
  rdfs:label "propertyComplementOf";
  rdfs:comment "The property that determines that a property is the complement of another property.";
  rdfs:isDefinedBy mel:;
  rdfs:domain rdf:Property;
  rdfs:range rdf:Property
  .

mel:propertyChainOf a rdf:Property;
  rdfs:label "propertyChainOf";
  rdfs:comment "The property that determines the sequence of object or datatype properties that build a chain of steps from first step to last.";
  rdfs:isDefinedBy mel:;
  rdfs:domain rdf:Property;
  rdfs:range rdf:List
  .

mel:hasIsA a owl:AnnotationProperty;
  rdfs:label "hasIsA";
  rdfs:comment "The property that determines the 'is a' property for a class.";
  rdfs:isDefinedBy mel:;
  rdfs:domain rdfs:Class;
  rdfs:range mel:IsAProperty
  .

mel:necessaryThat a rdf:Property;
  rdfs:label "necessaryThat";
  rdfs:comment "The property that determines the class that is necessarily true.";
  rdfs:isDefinedBy mel:;
  rdfs:domain mel:AlethicModal;
  rdfs:range owl:Class
  .

mel:possibleThat a rdf:Property;
  rdfs:label "possibleThat";
  rdfs:comment "The property that determines the class that is possibly true.";
  rdfs:isDefinedBy mel:;
  rdfs:domain mel:AlethicModal;
  rdfs:range owl:Class
  .

mel:assumedThat a rdf:Property;
  rdfs:label "assumedThat";
  rdfs:comment "The property that determines the classification that is assumed true (uses the OWA).";
  rdfs:isDefinedBy mel:;
  rdfs:domain mel:EpistemicModal;
  rdfs:range owl:Class
  .

mel:assertedThat a rdf:Property;
  rdfs:label "assertedThat";
  rdfs:comment "The property that determines the classification that is asserted true (uses the CWA).";
  rdfs:isDefinedBy mel:;
  rdfs:domain mel:EpistemicModal;
  rdfs:range owl:Class
  .

mel:provenThat a rdf:Property;
  rdfs:label "provenThat";
  rdfs:comment "The property that determines the classification that is asserted true (uses the CWA) with a suitable proof certificate for the assertions.";
  rdfs:isDefinedBy mel:;
  rdfs:domain mel:EpistemicModal;
  rdfs:range owl:Class
  .

mel:seesToItThat a rdf:Property;
  rdfs:label "seesToItThat";
  rdfs:comment "The property that determines the classification that is made true by the agent's actions.";
  rdfs:isDefinedBy mel:;
  rdfs:domain mel:DeonticModal;
  rdfs:range owl:Class
  .

mel:agentRestriction a rdf:Property;
  rdfs:label "agentRestriction";
  rdfs:comment "The property that determines the class of agents that are responsible for making the classification true.";
  rdfs:isDefinedBy mel:;
  rdfs:domain mel:DeonticModal;
  rdfs:range owl:Class
  .

mel:onCondition a rdf:Property;
  rdfs:label "onCondition";
  rdfs:comment "The property that determines the classification that must apply for this modal to also apply.";
  rdfs:isDefinedBy mel:;
  rdfs:domain mel:ModalRestriction;
  rdfs:range owl:Class
  .

owl:ObjectVariable a rdfs:Class;
  rdfs:label "ObjectVariable";
  rdfs:comment "The class of object (nominal) variables.";
  rdfs:isDefinedBy mel:;
  rdfs:subClassOf owl:Class
  .

owl:variableId a owl:DatatypeProperty;
  rdfs:label "variableId";
  rdfs:comment "The property that determines the variable identifier for an object variable";
  rdfs:isDefinedBy mel:;
  rdfs:domain owl:ObjectVariable;
  rdfs:range xsd:string
  .